Cleaning up the reasoning on binders. Trashed the obsolete freshness theory

coq/LLVMGen/StateCounters.v
@@ -1,3 +1,10 @@
+(** * Compilation units and IRState
+
+    This file contains a bunch of lemmas describing how various compilation subroutines
+    impact the [IRStated].
+
+ *)
+
 Require Import Helix.LLVMGen.Correctness_Prelude.
 
 Import ListNotations.
@@ -5,6 +12,7 @@ Import ListNotations.
 Set Implicit Arguments.
 Set Strict Implicit.
 
+Transparent resolve_PVar.
 (* TODO: Not sure where this should belong *)
 Lemma resolve_PVar_simple : forall p s s' x v,
     resolve_PVar p s ≡ inr (s', (x, v)) ->
@@ -22,7 +30,6 @@ Qed.
 Ltac inv_resolve_PVar H :=
   apply resolve_PVar_simple in H;
   destruct H as (?sz & ?n & ?LUn & ?EQsz & -> & <-).
-
 
 Global Opaque resolve_PVar.
 
@@ -67,3 +74,344 @@ Proof.
   destruct H0 as (sz & n & H0).
   intuition.
 Qed.
+
+Lemma incBlockNamed_local_count:
+  forall s s' msg id,
+    incBlockNamed msg s ≡ inr (s', id) ->
+    local_count s' ≡ local_count s.
+Proof.
+  intros; cbn in *; inv_sum; reflexivity.
+Qed.
+
+Lemma incVoid_local_count:
+  forall s s' id,
+    incVoid s ≡ inr (s', id) ->
+    local_count s' ≡ local_count s.
+Proof.
+  Transparent incVoid.
+  intros; cbn in *; inv_sum; reflexivity.
+  Opaque incVoid.
+Qed.
+
+Lemma incLocal_local_count: forall s s' x,
+    incLocal s ≡ inr (s',x) ->
+    local_count s' ≡ S (local_count s).
+Proof.
+  Transparent incLocal.
+  intros; cbn in *; inv_sum; reflexivity.
+  Opaque incLocal.
+Qed.
+
+Lemma incLocalNamed_local_count: forall s s' msg x,
+    incLocalNamed msg s ≡ inr (s',x) ->
+    local_count s' ≡ S (local_count s).
+Proof.
+  intros; cbn in *; inv_sum; reflexivity.
+Qed.
+
+(* We define the obvious total order on IRStates *)
+Definition IRState_lt (s1 s2 : IRState) : Prop :=
+  (local_count s1 < local_count s2)%nat.
+Infix "<<" := IRState_lt (at level 10).
+
+Definition IRState_le (s1 s2 : IRState) : Prop :=
+  (local_count s1 <= local_count s2)%nat.
+Infix "<<=" := IRState_le (at level 10).
+
+Lemma incLocal_lt : forall s1 s2 x,
+    incLocal s1 ≡ inr (s2,x) ->
+    s1 << s2.
+Proof.
+  intros s1 s2 x INC.
+  apply incLocal_local_count in INC.
+  unfold IRState_lt.
+  lia.
+Qed.
+
+Create HintDb irs_lt.
+Hint Resolve incLocal_lt : irs_lt.
+
+Lemma genNExpr_local_count :
+  forall nexp s1 s2 e c,
+    genNExpr nexp s1 ≡ inr (s2, (e, c)) ->
+    (local_count s2 >= local_count s1)%nat.
+Proof.
+  induction nexp;
+    intros s1 s2 e c GEN;
+    cbn* in *; simp; cbn in *;
+      repeat
+        match goal with
+        | H : incLocal ?s1 ≡ inr (?s2, _) |- _ =>
+          apply incLocal_local_count in H
+        | IH : ∀ (s1 s2 : IRState) (e : exp typ) (c : code typ),
+            genNExpr ?n s1 ≡ inr (s2, (e, c)) → local_count s2 ≥ local_count s1,
+    GEN: genNExpr ?n _ ≡ inr _ |- _ =>
+  apply IH in GEN
+  end;
+    try lia.
+Qed.
+
+Lemma genMExpr_local_count :
+  forall mexp s1 s2 e c,
+    genMExpr mexp s1 ≡ inr (s2, (e, c)) ->
+    (local_count s2 >= local_count s1)%nat.
+Proof.
+  induction mexp;
+    intros s1 s2 e c GEN;
+    cbn* in *; simp; cbn in *;
+      repeat
+        match goal with
+        | H : incLocal ?s1 ≡ inr (?s2, _) |- _ =>
+          apply incLocal_local_count in H
+        | IH : ∀ (s1 s2 : IRState) (e : exp typ) (c : code typ),
+            genMExpr ?n s1 ≡ inr (s2, (e, c)) → local_count s2 ≥ local_count s1,
+    GEN: genMExpr ?n _ ≡ inr _ |- _ =>
+  apply IH in GEN
+  end;
+    try lia.
+Qed.
+
+Lemma genAExpr_local_count :
+  forall aexp s1 s2 e c,
+    genAExpr aexp s1 ≡ inr (s2, (e, c)) ->
+    (local_count s2 >= local_count s1)%nat.
+Proof.
+  induction aexp;
+    intros s1 s2 e c GEN;
+    cbn* in *; simp; cbn in *;
+      repeat
+        match goal with
+        | H : incLocal ?s1 ≡ inr (?s2, _) |- _ =>
+          apply incLocal_local_count in H
+        | H : incVoid ?s1 ≡ inr (?s2, _) |- _ =>
+          apply incVoid_local_count in H
+        | GEN : genNExpr _ _ ≡ inr _ |- _ =>
+          apply genNExpr_local_count in GEN
+        | GEN : genMExpr _ _ ≡ inr _ |- _ =>
+          apply genMExpr_local_count in GEN
+        | IH : ∀ (s1 s2 : IRState) (e : exp typ) (c : code typ),
+            genAExpr ?a s1 ≡ inr _ → local_count s2 ≥ local_count s1,
+    GEN : genAExpr ?a _ ≡ inr _ |- _ =>
+  apply IH in GEN
+  end; try lia.
+Qed.
+
+Arguments append: simpl never.
+Opaque incBlockNamed.
+Opaque incVoid.
+Opaque incLocal.
+
+Ltac __local_ltac :=
+  repeat
+    (match goal with
+     | H: inl _ ≡ inr _ |- _ =>
+       inversion H
+     | H: ErrorWithState.option2errS _ (nth_error (Γ ?s1) ?n) ?s1 ≡ inr (?s2, _) |- _ =>
+       destruct (nth_error (Γ s1) n) eqn:?; inversion H; subst
+     | H : ErrorWithState.err2errS (MInt64asNT.from_nat ?n) ?s1 ≡ inr (?s2, _) |- _ =>
+       destruct (MInt64asNT.from_nat n) eqn:?; inversion H; subst
+     | H : incLocal ?s1 ≡ inr (?s2, _) |- _ =>
+       apply incLocal_local_count in H
+     | H : incVoid ?s1 ≡ inr (?s2, _) |- _ =>
+       apply incVoid_local_count in H
+     | H : incBlockNamed _ _ ≡ inr _ |- _ =>
+       apply incBlockNamed_local_count in H
+     | H : incBlock _ ≡ inr _ |- _ =>
+       apply incBlockNamed_local_count in H
+     | H : resolve_PVar _ _ ≡ inr _ |- _ =>
+       apply resolve_PVar_state in H; subst
+     | GEN : genNExpr _ _ ≡ inr _ |- _ =>
+       apply genNExpr_local_count in GEN
+     | GEN : genMExpr _ _ ≡ inr _ |- _ =>
+       apply genMExpr_local_count in GEN
+     | GEN : genAExpr _ _ ≡ inr _ |- _ =>
+       apply genAExpr_local_count in GEN
+     | IH : ∀ (s1 s2 : IRState) (nextblock b : block_id) (bk_op : list (LLVMAst.block typ)),
+         genIR ?op nextblock s1 ≡ inr (s2, (b, bk_op)) → local_count s2 ≥ local_count s1,
+       GEN: genIR ?op _ _ ≡ inr _ |- _ =>
+     apply IH in GEN
+     end; cbn in *).
+
+Lemma genIR_local_count :
+  forall op s1 s2 nextblock b bk_op,
+    genIR op nextblock s1 ≡ inr (s2, (b, bk_op)) ->
+    local_count s2 ≥ local_count s1.
+Proof.
+  induction op; intros; cbn in H; simp; __local_ltac; lia. 
+Qed.
+
+
+Lemma genNExpr_block_count :
+  ∀ (nexp : NExpr) (s1 s2 : IRState) (e : exp typ) (c : code typ),
+    genNExpr nexp s1 ≡ inr (s2, (e, c)) → (block_count s2 ≡ block_count s1)%nat.
+Proof.
+  induction nexp;
+    intros s1 s2 e c GEN;
+    cbn in GEN; simp; cbn;
+      repeat
+        match goal with
+        | H: ErrorWithState.option2errS _ (nth_error (Γ ?s1) ?n) ?s1 ≡ inr (?s2, _) |- _ =>
+          destruct (nth_error (Γ s1) n) eqn:FIND; inversion H; subst
+        | H : incLocal ?s1 ≡ inr (?s2, _) |- _ =>
+          apply incLocal_block_count in H
+        | IH : ∀ (s1 s2 : IRState) (e : exp typ) (c : code typ),
+            genNExpr ?n s1 ≡ inr (s2, (e, c)) → block_count s2 ≡ block_count s1,
+    GEN: genNExpr ?n _ ≡ inr _ |- _ =>
+  apply IH in GEN
+  end; subst; auto; try lia.
+Qed.
+
+(* TODO: Move this *)
+Lemma genMExpr_block_count :
+  ∀ (mexp : MExpr) (s1 s2 : IRState) (e : exp typ * code typ) (c : typ),
+    genMExpr mexp s1 ≡ inr (s2, (e, c)) → block_count s2 ≡ block_count s1.
+Proof.
+  induction mexp;
+    intros s1 s2 e c GEN;
+    cbn in GEN; simp; cbn;
+      repeat
+        match goal with
+        | H: ErrorWithState.option2errS _ (nth_error (Γ ?s1) ?n) ?s1 ≡ inr (?s2, _) |- _ =>
+          destruct (nth_error (Γ s1) n) eqn:FIND; inversion H; subst
+        | H : incLocal ?s1 ≡ inr (?s2, _) |- _ =>
+          apply incLocal_block_count in H
+        | IH : ∀ (s1 s2 : IRState) (e : exp typ) (c : code typ),
+            genMExpr ?n s1 ≡ inr (s2, (e, c)) → block_count s2 ≡ block_count s1,
+    GEN: genMExpr ?n _ ≡ inr _ |- _ =>
+  apply IH in GEN
+  end; subst; auto; try lia.
+Qed.
+
+(* TODO: Move this *)
+Lemma genAExpr_block_count :
+  ∀ (aexp : AExpr) (s1 s2 : IRState) (e : exp typ) (c : code typ),
+    genAExpr aexp s1 ≡ inr (s2, (e, c)) → block_count s2 ≡ block_count s1.
+Proof.
+  induction aexp;
+    intros s1 s2 e c GEN;
+    cbn in GEN; simp; cbn;
+      repeat
+        match goal with
+        | H: ErrorWithState.option2errS _ (nth_error (Γ ?s1) ?n) ?s1 ≡ inr (?s2, _) |- _ =>
+          destruct (nth_error (Γ s1) n) eqn:FIND; inversion H; subst
+        | H : incLocal ?s1 ≡ inr (?s2, _) |- _ =>
+          apply incLocal_block_count in H
+        | H : incVoid ?s1 ≡ inr (?s2, _) |- _ =>
+          apply incVoid_block_count in H
+        | GEN : genNExpr _ _ ≡ inr _ |- _ =>
+          apply genNExpr_block_count in GEN
+        | GEN : genMExpr _ _ ≡ inr _ |- _ =>
+          apply genMExpr_block_count in GEN
+        | IH : ∀ (s1 s2 : IRState) (e : exp typ) (c : code typ),
+            genAExpr ?n s1 ≡ inr (s2, (e, c)) → block_count s2 ≡ block_count s1,
+    GEN: genAExpr ?n _ ≡ inr _ |- _ =>
+  apply IH in GEN
+  end; subst; auto; try lia.
+Qed.
+
+Transparent incBlockNamed.
+Lemma incBlockNamed_Γ:
+  forall s s' msg id,
+    incBlockNamed msg s ≡ inr (s', id) ->
+    Γ s' ≡ Γ s.
+Proof.
+  intros; cbn in *; inv_sum; reflexivity.
+Qed.
+
+Lemma incBlockNamed_block_count:
+  forall s s' msg id,
+    incBlockNamed msg s ≡ inr (s', id) ->
+    block_count s' ≡ S (block_count s).
+Proof.
+  intros; cbn in *; inv_sum; reflexivity.
+Qed.
+Opaque incBlockNamed.
+
+Ltac __local_ltac' :=
+  repeat
+    (match goal with
+     | H: inl _ ≡ inr _ |- _ =>
+       inversion H
+     | H: ErrorWithState.option2errS _ (nth_error (Γ ?s1) ?n) ?s1 ≡ inr (?s2, _) |- _ =>
+       destruct (nth_error (Γ s1) n) eqn:?; inversion H; subst
+     | H : ErrorWithState.err2errS (MInt64asNT.from_nat ?n) ?s1 ≡ inr (?s2, _) |- _ =>
+       destruct (MInt64asNT.from_nat n) eqn:?; inversion H; subst
+     | H : incLocal ?s1 ≡ inr (?s2, _) |- _ =>
+       apply incLocal_block_count in H
+     | H : incVoid ?s1 ≡ inr (?s2, _) |- _ =>
+       apply incVoid_block_count in H
+     | H : incBlockNamed _ _ ≡ inr _ |- _ =>
+       apply incBlockNamed_block_count in H
+     | H : incBlock _ ≡ inr _ |- _ =>
+       apply incBlockNamed_block_count in H
+     | H : resolve_PVar _ _ ≡ inr _ |- _ =>
+       apply resolve_PVar_state in H; subst
+     | GEN : genNExpr _ _ ≡ inr _ |- _ =>
+       apply genNExpr_block_count in GEN
+     | GEN : genMExpr _ _ ≡ inr _ |- _ =>
+       apply genMExpr_block_count in GEN
+     | GEN : genAExpr _ _ ≡ inr _ |- _ =>
+       apply genAExpr_block_count in GEN
+     | IH : ∀ (s1 s2 : IRState) (nextblock b : block_id) (bk_op : list (LLVMAst.block typ)),
+         genIR ?op nextblock s1 ≡ inr (s2, (b, bk_op)) → block_count s2 ≥ block_count s1,
+       GEN: genIR ?op _ _ ≡ inr _ |- _ =>
+     apply IH in GEN
+     end; cbn in *).
+
+Lemma genIR_block_count :
+  forall op s1 s2 nextblock b bk_op,
+    genIR op nextblock s1 ≡ inr (s2, (b, bk_op)) ->
+    block_count s2 ≥ block_count s1.
+Proof.
+  induction op; intros; cbn in H; simp; __local_ltac'; lia. 
+Qed.
+
+Transparent incBlockNamed.
+Transparent incVoid.
+Transparent incLocal.
+
+(* Tactics *)
+
+Ltac get_local_count_hyps :=
+  repeat
+    match goal with
+    | H: incBlockNamed ?n ?s1 ≡ inr (?s2, _) |- _ =>
+      apply incBlockNamed_local_count in H
+    | H: incLocalNamed ?n ?s1 ≡ inr (?s2, _) |- _ =>
+      apply incLocalNamed_local_count in H
+    | H: incVoid ?s1 ≡ inr (?s2, _) |- _ =>
+      apply incVoid_local_count in H
+    | H: incLocal ?s1 ≡ inr (?s2, _) |- _ =>
+      apply incLocal_local_count in H
+    | H: genNExpr ?n ?s1 ≡ inr (?s2, _) |- _ =>
+      apply genNExpr_local_count in H
+    | H: genMExpr ?m ?s1 ≡ inr (?s2, _) |- _ =>
+      apply genMExpr_local_count in H
+    | H: genAExpr ?a ?s1 ≡ inr (?s2, _) |- _ =>
+      apply genAExpr_local_count in H
+    | H: genIR ?op ?id ?s1 ≡ inr (?s2, _) |- _ =>
+      apply genIR_local_count in H
+    end.
+
+Ltac solve_local_count_tac := try solve [unfold IRState_lt, IRState_le in *; get_local_count_hyps; lia].
+
+Ltac solve_local_count :=
+  match goal with
+  | |- (local_count ?s1 > local_count ?s2)%nat =>
+    solve_local_count_tac
+  | |- (local_count ?s1 < local_count ?s2)%nat =>
+    solve_local_count_tac
+  | |- (local_count ?s1 >= local_count ?s2)%nat =>
+    solve_local_count_tac
+  | |- (local_count ?s1 <= local_count ?s2)%nat =>
+    solve_local_count_tac
+  | |- ?s1 << ?s2 =>
+    solve_local_count_tac
+  | |- ?s1 <<= ?s2 =>
+    solve_local_count_tac
+  | |- local_count ?s1 ≡ local_count ?s2 =>
+    solve_local_count_tac
+  | |- local_count ?s1 ≢ local_count ?s2 =>
+    solve_local_count_tac
+  end.
+
